lib/pipeline.ml
@@ -49,7 +49,9 @@ struct
   (* Must track [alloc_idents] in theories/compiler/dfa.v. *)
   reg 0 "delta" ;
   reg 1 "accept" ;
-  reg 2 "q0" 
+  reg 2 "q0" ;
+  reg 3 "table" ;
+  reg 9 "run"
 
   (** Compile the learned DFA to Clight and print it to [output_fn] or [stdout]
 
