theories/transparency/dfa.v
@@ -1,7 +1,7 @@
 From lstar Require Import Automata.
 From compcert Require Import AST Clight Ctypes Integers Cop Maps.
 From compcert Require Import ClightBigstep Values Events Coqlib.
-From compcert Require Import Globalenvs.
+From compcert Require Import Globalenvs Memory.
 From Transmogrifier Require Import Monads.
 From Transmogrifier.compiler Require Import dfa.
 From Stdlib Require Import List ZArith Lia.
@@ -174,10 +174,12 @@ Definition ids : idents := alloc_idents base.
 
 Lemma compile_program_defs :
   prog_defs p =
-    [ (ids.(id_delta),  Gfun (compile_delta state dfa state_eq_dec ids));
+    [ (ids.(id_table),  Gvar (compile_table state dfa state_eq_dec));
+      (ids.(id_delta),  Gfun (compile_delta state dfa ids));
       (ids.(id_accept), Gfun (compile_accept state dfa ids));
       (ids.(id_q0),     Gvar (compile_q0 state dfa state_eq_dec));
-      (ids.(id_run),    Gfun (compile_run state dfa state_eq_dec ids)) ].
+      (ids.(id_run),    Gfun (compile_run state dfa state_eq_dec ids));
+      (ids.(id_main),   Gfun (compile_main ids)) ].
 Proof.
   unfold ids. unfold compile_program in Hp.
   destruct Ctypes.make_program eqn:E; [|discriminate].
@@ -198,28 +200,43 @@ Qed.
 
 Lemma compile_program_defs_ast :
   AST.prog_defs (program_of_program p) =
-    [ (ids.(id_delta),  Gfun (compile_delta state dfa state_eq_dec ids));
+    [ (ids.(id_table),  Gvar (compile_table state dfa state_eq_dec));
+      (ids.(id_delta),  Gfun (compile_delta state dfa ids));
       (ids.(id_accept), Gfun (compile_accept state dfa ids));
       (ids.(id_q0),     Gvar (compile_q0 state dfa state_eq_dec));
-      (ids.(id_run),    Gfun (compile_run state dfa state_eq_dec ids)) ].
+      (ids.(id_run),    Gfun (compile_run state dfa state_eq_dec ids));
+      (ids.(id_main),   Gfun (compile_main ids)) ].
 Proof. exact compile_program_defs. Qed.
 
 Lemma defmap_delta :
   (prog_defmap p) ! (ids.(id_delta)) =
-    Some (Gfun (compile_delta state dfa state_eq_dec ids)).
+    Some (Gfun (compile_delta state dfa ids)).
 Proof.
   unfold prog_defmap. rewrite compile_program_defs_ast.
   apply PTree_Properties.of_list_norepet.
     rewrite <- compile_program_defs. apply global_idents_norepet.
-  now left.
+  right. now left.
 Qed.
 
 Lemma find_delta_def :
   exists b,
     Genv.find_symbol ge ids.(id_delta) = Some b /\
-    Genv.find_def ge b = Some (Gfun (compile_delta state dfa state_eq_dec ids)).
+    Genv.find_def ge b = Some (Gfun (compile_delta state dfa ids)).
 Proof.
   apply Genv.find_def_symbol. apply defmap_delta.
+Qed.
+
+Lemma find_delta :
+  exists b,
+    Genv.find_symbol ge ids.(id_delta) = Some b /\
+    Genv.find_funct ge (Vptr b Ptrofs.zero) =
+      Some (compile_delta state dfa ids).
+Proof.
+  destruct find_delta_def as (b & Hsym & Hdef).
+  exists b. split.
+    assumption.
+  unfold Genv.find_funct. rewrite pred_dec_true by reflexivity.
+  now apply Genv.find_funct_ptr_iff.
 Qed.
 
 (* index of a state *)
@@ -281,6 +298,18 @@ Proof.
   destruct Archi.ptr64; cbn; rewrite Int.eq_true; reflexivity.
 Qed.
 
+Lemma bool_val_one_int : forall m, bool_val (Vint Int.one) tint m = Some true.
+Proof.
+  intros m. unfold bool_val, tint. cbn.
+  destruct Archi.ptr64; cbn; rewrite Int.eq_false by apply Int.one_not_zero; reflexivity.
+Qed.
+
+Lemma bool_val_zero_int : forall m, bool_val (Vint Int.zero) tint m = Some false.
+Proof.
+  intros m. unfold bool_val, tint. cbn.
+  destruct Archi.ptr64; cbn; rewrite Int.eq_true; reflexivity.
+Qed.
+
 Lemma fold_left_preserves_head : forall (A B : Type) (f : A -> B -> A) (P : A -> Prop) (l : list B) (a : A),
   P a ->
   (forall x b, In b l -> P x -> P (f x b)) ->
@@ -293,79 +322,168 @@ Proof.
   intros. apply H0. now right. assumption.
 Qed.
 
-Lemma sym_branch_exec : forall ids e le m tbl acc q sym s_idx next_idx,
-  le ! (ids.(id_s)) = Some (Vlong (Int64.repr s_idx)) ->
-  sidx (dfa.(transition _) q sym) = Some next_idx ->
-  In (s_idx, sym) tbl ->
-  (forall i a, In (i, a) tbl -> 0 <= i < Int64.modulus) ->
-  list_norepet (map fst tbl) ->
-  exec_stmt function_entry2 ge e le m
-    (fold_left (fun (acc : statement) '(si, sy) =>
-       match sidx (dfa.(transition _) q sy) with
-       | Some ni => Sifthenelse (eq_test ids.(id_s) si)
-                      (Sreturn (Some (Econst_long (Int64.repr ni) tlong)))
-                      acc
-       | None => acc
-       end) tbl acc)
-    E0 le m (Out_return (Some (Vlong (Int64.repr next_idx), tlong))).
-Proof.
-  induction tbl; intros; simpl in *. contradiction.
-  inversion H3; subst; clear H3.
-  destruct H1; subst.
-  - (* head is the matching entry: si = s_idx, sy = sym *)
-    rewrite H0. apply fold_left_preserves_head.
-    + econstructor.
-        eauto using eval_eq_test_true.
-        apply bool_val_one.
-        simpl. econstructor. econstructor.
-    + intros. destruct b as (si & sy), (sidx (transition state dfa q sy)) eqn:E; auto.
-      econstructor.
-        eapply eval_eq_test_false; eauto.
-          intro. subst. apply H6. simpl.
-          change si with (fst (si, sy)).
-          now apply in_map.
-        apply bool_val_zero.
-        assumption.
-  - (* the match is later in the table *)
-    destruct a as (si & sy), (sidx (dfa.(transition _) q sy)) eqn:E;
-      eapply IHtbl; eauto; intros; eapply H2; right; eassumption.
+(* delta lookup table *)
+
+Lemma nth_error_flat_map_uniform :
+  forall (A B : Type) (f : A -> list B) (l : list A) (k : nat),
+  (forall x, In x l -> length (f x) = k) ->
+  forall i j x,
+  nth_error l i = Some x ->
+  (j < k)%nat ->
+  nth_error (flat_map f l) (i * k + j) = nth_error (f x) j.
+Proof. clear.
+  induction l; intros k Hk i j x Hi Hj; simpl in *.
+    now destruct i.
+  destruct i; simpl in *.
+  - (* head row: index j lands inside (f a) *)
+    inversion Hi; subst; clear Hi.
+    rewrite nth_error_app1.
+      reflexivity.
+    rewrite Hk by now left. assumption.
+  - (* later row: skip past (f a), which has length k *)
+    rewrite nth_error_app2.
+      rewrite Hk by now left.
+      replace (k + i * k + j - k)%nat with (i * k + j)%nat by lia. eauto.
+    rewrite Hk. lia. now left.
 Qed.
 
-(** The state branch tree *)
+Lemma enumerate_nth_error_pair : forall (X : Type) (l : list X) i,
+  0 <= i < Z.of_nat (length l) ->
+  exists x, nth_error (enumerate l) (Z.to_nat i) = Some (i, x)
+            /\ nth_error l (Z.to_nat i) = Some x.
+Proof.
+  intros. unfold enumerate.
+  destruct (nth_error l (Z.to_nat i)) eqn:E.
+  - exists x. split; [|reflexivity].
+    rewrite nth_error_combine, E, nth_error_map, nth_error_seq.
+    cbn. replace (match Datatypes.length l with
+           | 0%nat => false
+           | S m' => (Z.to_nat i <=? m')%nat
+           end) with true.
+      cbn. now rewrite Z2Nat.id by lia.
+    symmetry. destruct (Datatypes.length l) eqn:El.
+      lia.
+    apply Nat.leb_le. lia.
+  - exfalso. apply nth_error_None in E. lia.
+Qed.
 
-Lemma delta_tree_exec : forall ids e le m tbl acc q sym q_idx s_idx next_idx,
-  le ! (ids.(id_q)) = Some (Vlong (Int64.repr q_idx)) ->
-  le ! (ids.(id_s)) = Some (Vlong (Int64.repr s_idx)) ->
+Lemma table_row_length : forall q,
+  length (table_row state dfa state_eq_dec q) = length s.enum.
+Proof.
+  intros. unfold table_row, sym_table, enumerate.
+  rewrite length_map, length_combine, length_map, length_seq. lia.
+Qed.
+
+Lemma table_entry_correct : forall q sym q_idx s_idx,
   sidx q = Some q_idx ->
   symidx sym = Some s_idx ->
-  sidx (dfa.(transition _) q sym) = Some next_idx ->
-  In (q_idx, q) tbl ->
-  (forall i x, In (i, x) tbl -> 0 <= i < Int64.modulus) ->
-  list_norepet (map fst tbl) ->
-  exec_stmt function_entry2 ge e le m
-    (fold_left (fun (acc : statement) '(qi, qq) =>
-       Sifthenelse (eq_test ids.(id_q) qi) (sym_branch state dfa ids state_eq_dec qi qq) acc)
-       tbl acc)
-    E0 le m (Out_return (Some (Vlong (Int64.repr next_idx), tlong))).
+  nth_error (table_init state dfa state_eq_dec)
+    (Z.to_nat (q_idx * nsyms + s_idx))
+  = Some (Init_int64 (Int64.repr (table_entry state dfa state_eq_dec q sym))).
 Proof.
-  induction tbl; intros; simpl in *. contradiction.
-  inversion H6; subst; clear H6. destruct H4; subst.
-  - apply fold_left_preserves_head.
-      econstructor.
-        eapply eval_eq_test_true; eauto.
-        apply bool_val_one.
-        simpl. unfold sym_branch.
-        eapply sym_branch_exec; eauto.
-          eapply enumerate_spec; eauto.
-          intros. pose proof (enumerate_In_bounds _ _ _ _ H4). lia.
-          apply enumerate_index_norepet.
-        intros. destruct b as (qi & qq). econstructor.
-          eapply eval_eq_test_false; eauto.
-            intro. subst. apply H9. simpl.
-            change qi with (fst (qi, qq)). now apply in_map.
-          apply bool_val_zero.
-        assumption.
-  - eapply IHtbl; eauto.
+  intros q sym q_idx s_idx Hq Hs.
+  assert (Hqb : 0 <= q_idx < Z.of_nat (length dfa.(states _)))
+    by (unfold sidx in Hq; eauto using index_of_bounds).
+  assert (Hsb : 0 <= s_idx < Z.of_nat (length s.enum))
+    by (unfold symidx in Hs; eauto using index_of_bounds).
+  (* the q_idx-th row of state_table is (q_idx, q) *)
+  assert (Hrow : nth_error (state_table state dfa) (Z.to_nat q_idx) = Some (q_idx, q)).
+    { unfold state_table.
+      destruct (enumerate_nth_error_pair _ (states state dfa) q_idx Hqb)
+        as (q' & Hpair & Hnth).
+      unfold sidx in Hq. apply index_of_nth_error in Hq.
+      rewrite Z.sub_0_r in Hq. rewrite Hq in Hnth.
+      inversion Hnth; subst. exact Hpair. }
+  (* the s_idx-th entry of the row is delta q sym *)
+  assert (Hcol : nth_error (table_row state dfa state_eq_dec q) (Z.to_nat s_idx)
+                 = Some (Init_int64 (Int64.repr (table_entry state dfa state_eq_dec q sym)))).
+    { unfold table_row, sym_table.
+      rewrite nth_error_map.
+      destruct (enumerate_nth_error_pair _ s.enum s_idx Hsb)
+        as (sym' & Hpair & Hnth).
+      unfold symidx in Hs. apply index_of_nth_error in Hs.
+      rewrite Z.sub_0_r in Hs. rewrite Hs in Hnth.
+      inversion Hnth; subst.
+      now rewrite Hpair. }
+  unfold table_init.
+  replace (Z.to_nat (q_idx * nsyms + s_idx))
+    with (Z.to_nat q_idx * length s.enum + Z.to_nat s_idx)%nat
+    by (unfold nsyms; lia).
+  rewrite nth_error_flat_map_uniform with (k := length s.enum) (x := (q_idx, q)).
+  - exact Hcol.
+  - intros (qi & qq) _. apply table_row_length.
+  - exact Hrow.
+  - lia.
+Qed.
+
+Variable m0 : mem.
+Variable Hinit : Genv.init_mem p = Some m0.
+
+Lemma find_table :
+  exists b,
+    Genv.find_symbol ge ids.(id_table) = Some b /\
+    Genv.find_def ge b = Some (Gvar (compile_table state dfa state_eq_dec)).
+Proof.
+  apply Genv.find_def_symbol.
+  apply prog_defmap_norepet.
+    apply global_idents_norepet.
+  pose proof compile_program_defs as Hdefs.
+  change (AST.prog_defs p) with (prog_defs p).
+  rewrite Hdefs. now left.
+Qed.
+
+Lemma init_data_list_nth_load :
+  forall (F V : Type) (ge' : Genv.t F V) b il n v m base_ofs,
+  (forall id, In id il -> exists x, id = Init_int64 x) ->
+  Genv.load_store_init_data ge' m b base_ofs il ->
+  nth_error il n = Some (Init_int64 v) ->
+  Mem.load Mint64 m b (base_ofs + 8 * Z.of_nat n) = Some (Vlong v).
+Proof. clear.
+  induction il; intros n v m base_ofs Hall Hlsid Hnth.
+    now destruct n.
+  destruct n; cbn - [Z.of_nat Z.mul] in *.
+  - inversion Hnth; subst; clear Hnth.
+    destruct Hlsid as (Hload & _).
+    now rewrite Z.add_0_r.
+  - destruct (Hall a) as (x & Hx); [now left|]. subst a.
+    destruct Hlsid as (_ & Hrest). cbn - [Z.of_nat] in Hrest.
+    replace (base_ofs + 8 * Z.of_nat (S n))
+      with ((base_ofs + 8) + 8 * Z.of_nat n) by lia.
+    eapply IHil; eauto.
+Qed.
+
+Lemma table_init_all_int64 : forall id,
+  In id (table_init state dfa state_eq_dec) -> exists x, id = Init_int64 x.
+Proof.
+  intros. unfold table_init in H.
+  apply in_flat_map in H. destruct H as ((qi & q) & _ & Hin).
+  unfold table_row in Hin. apply in_map_iff in Hin.
+  destruct Hin as ((si & sy) & Heq & _). subst. eauto.
+Qed.
+
+Variable table_bounded : 8 * (Z.of_nat (length dfa.(states _)) * Z.of_nat (length s.enum))
+                         < Ptrofs.modulus.
+
+Lemma table_in_mem : forall b k v,
+  Genv.find_symbol ge ids.(id_table) = Some b ->
+  nth_error (table_init state dfa state_eq_dec) (Z.to_nat k) = Some (Init_int64 v) ->
+  0 <= k < (nstates state dfa) * nsyms ->
+  Mem.loadv Mint64 m0 (Vptr b (Ptrofs.repr (8 * k))) = Some (Vlong v).
+Proof.
+  intros b k v Hsym Hnth Hk.
+  destruct find_table as (b' & Hsym' & Hdef).
+  assert (b' = b) by congruence. subst b'.
+  assert (Hvi : Genv.find_var_info ge b = Some (compile_table state dfa state_eq_dec)).
+    { apply Genv.find_var_info_iff. exact Hdef. }
+  destruct (Genv.init_mem_characterization _ _ Hvi Hinit)
+    as (_ & _ & Hlsid & _).
+  specialize (Hlsid eq_refl).
+  cbn [Mem.loadv].
+  rewrite Ptrofs.unsigned_repr.
+  - replace (8 * k) with (0 + 8 * Z.of_nat (Z.to_nat k)) by lia.
+    eapply init_data_list_nth_load; eauto.
+    apply table_init_all_int64.
+  - unfold Ptrofs.max_unsigned. unfold nstates, nsyms in Hk. lia.
 Qed.
 
 Lemma alloc_idents_norepet : forall base,
@@ -375,36 +493,185 @@ Proof.
   repeat constructor. intros [H|[]]. lia. now intro.
 Qed.
 
+Lemma eval_lt_test_gen : forall e le m v j k bv,
+  le ! v = Some (Vlong (Int64.repr j)) ->
+  0 <= j < Int64.modulus -> 0 <= k < Int64.modulus ->
+  bv = (if j <? k then Int.one else Int.zero) ->
+  eval_expr ge e le m (lt_test v k) (Vint bv).
+Proof.
+  intros. unfold lt_test. econstructor.
+    econstructor. eassumption.
+    econstructor.
+  cbn. unfold sem_cmp, classify_cmp, tlong, sem_binarith, sem_cast,
+              classify_cast, classify_binarith. cbn.
+  destruct Archi.ptr64; cbn;
+    unfold Val.of_bool, Int64.ltu;
+    repeat rewrite Int64.unsigned_repr by (unfold Int64.max_unsigned; lia);
+    subst; destruct (j <? k) eqn:E;
+      [ rewrite zlt_true by lia | rewrite zlt_false by lia
+      | rewrite zlt_true by lia | rewrite zlt_false by lia ];
+      reflexivity.
+Qed.
+
+Lemma nsyms_bound : 0 <= DC.nsyms <= Int64.max_unsigned.
+Proof.
+  unfold DC.nsyms, Int64.max_unsigned.
+  pose proof (Nat2Z.is_nonneg (Datatypes.length s.enum)). lia.
+Qed.
+
+Lemma nstates_bound : 0 <= DC.nstates state dfa <= Int64.max_unsigned.
+Proof.
+  unfold DC.nstates, Int64.max_unsigned.
+  pose proof (Nat2Z.is_nonneg (Datatypes.length (states state dfa))). lia.
+Qed.
+
+Lemma mul_repr_in_range : forall a b,
+  0 <= a <= Int64.max_unsigned -> 0 <= b <= Int64.max_unsigned ->
+  Int64.mul (Int64.repr a) (Int64.repr b) = Int64.repr (a * b).
+Proof.
+  intros. unfold Int64.mul. now rewrite !Int64.unsigned_repr by assumption.
+Qed.
+
+Lemma add_repr_in_range : forall a b,
+  0 <= a <= Int64.max_unsigned -> 0 <= b <= Int64.max_unsigned ->
+  Int64.add (Int64.repr a) (Int64.repr b) = Int64.repr (a + b).
+Proof.
+  intros. rewrite Int64.add_unsigned. now rewrite !Int64.unsigned_repr by assumption.
+Qed.
+
+Lemma ptrofs_le_int64 : Ptrofs.modulus <= Int64.modulus.
+Proof.
+  unfold Ptrofs.modulus, Int64.modulus, Ptrofs.wordsize, Int64.wordsize,
+         Wordsize_Ptrofs.wordsize, Wordsize_64.wordsize, two_power_nat.
+  destruct Archi.ptr64; cbn; lia.
+Qed.
+
+Lemma ptr_add_normalize : forall ofs i,
+  0 <= ofs -> 0 <= i -> ofs + 8 * i < Ptrofs.modulus ->
+  Ptrofs.add (Ptrofs.repr ofs)
+    (Ptrofs.mul (Ptrofs.repr 8) (Ptrofs.of_int64 (Int64.repr i)))
+  = Ptrofs.repr (ofs + 8 * i).
+Proof.
+  intros.
+  pose proof ptrofs_le_int64.
+  unfold Ptrofs.add, Ptrofs.mul, Ptrofs.of_int64.
+  rewrite Int64.unsigned_repr by (unfold Int64.max_unsigned; lia).
+  repeat rewrite Ptrofs.unsigned_repr_eq.
+  rewrite (Zmod_small ofs) by lia.
+  rewrite (Zmod_small i) by lia.
+  rewrite (Zmod_small 8).
+  - now rewrite (Zmod_small (8 * i)) by lia.
+  - unfold Ptrofs.modulus, Ptrofs.wordsize, Wordsize_Ptrofs.wordsize, two_power_nat.
+    destruct Archi.ptr64; cbn; lia.
+Qed.
+
+Lemma table_entry_sidx : forall q sym next_idx,
+  sidx (dfa.(transition _) q sym) = Some next_idx ->
+  table_entry state dfa state_eq_dec q sym = next_idx.
+Proof. intros. unfold table_entry, sidx in *. now rewrite H. Qed.
+
 (** delta is correct on valid indices *)
 
-Lemma compile_delta_correct :
-  forall base q sym q_idx s_idx next_idx m,
-    sidx q = Some q_idx ->
-    symidx sym = Some s_idx ->
-    sidx (dfa.(transition _) q sym) = Some next_idx ->
-    eval_funcall function_entry2 ge m
-      (compile_delta state dfa state_eq_dec (alloc_idents base))
-      [Vlong (Int64.repr q_idx); Vlong (Int64.repr s_idx)] E0 m
-      (Vlong (Int64.repr next_idx)).
+Lemma compile_delta_correct : forall q sym q_idx s_idx next_idx,
+  sidx q = Some q_idx ->
+  symidx sym = Some s_idx ->
+  sidx (dfa.(transition _) q sym) = Some next_idx ->
+  eval_funcall function_entry2 ge m0
+    (compile_delta state dfa ids)
+    [Vlong (Int64.repr q_idx); Vlong (Int64.repr s_idx)] E0 m0
+    (Vlong (Int64.repr next_idx)).
 Proof.
-  intros. unfold compile_delta.
-  econstructor.
-  - econstructor; cbn - [Pos.succ Pos.add]; try solve [constructor].
+  set (nstates := nstates state dfa).
+  intros. destruct find_table as (tb & Hsym & _).
+  assert (Hq : 0 <= q_idx < nstates) by (unfold sidx, nstates, DC.nstates in *; apply index_of_bounds in H; lia).
+  assert (Hs : 0 <= s_idx < nsyms) by (unfold symidx, nsyms, DC.nstates in *; apply index_of_bounds in H0; lia).
+  assert (Hprod : 0 <= q_idx * DC.nsyms + s_idx < DC.nstates state dfa * DC.nsyms).
+    { unfold DC.nstates, DC.nsyms in *. nia. }
+  assert (Hpb : 8 * (q_idx * DC.nsyms + s_idx) < Ptrofs.modulus).
+    { unfold DC.nstates, DC.nsyms in *. nia. }
+  econstructor; try easy.
+  - econstructor; cbn - [Pos.add]; try solve [constructor].
       apply alloc_idents_norepet.
       now repeat intro.
-  - cbn [fn_body].
-    eapply delta_tree_exec with (q := q) (sym := sym); eauto.
-    + cbn - [Pos.succ Pos.add].
-      rewrite PTree.gso by (unfold alloc_idents; cbn - [Pos.succ Pos.add]; lia).
-      rewrite PTree.gss. reflexivity.
-    + cbn - [Pos.succ]. rewrite PTree.gss. reflexivity.
-    + eauto using enumerate_spec.
-    + intros.
-      pose proof (enumerate_In_bounds _ _ _ _ H2). lia.
-    + apply enumerate_index_norepet.
+  - cbn [fn_body]. econstructor.
+    + (* guard: (q < |Q|) & (s < |Sigma|) evaluates to Int.one *)
+      econstructor.
+      * (* left conjunct *)
+        eapply eval_lt_test_gen with (j := q_idx) (bv := Int.one).
+        -- cbn - [Pos.add].
+           rewrite PTree.gso by (cbv [ids alloc_idents id_q id_s]; lia).
+           apply PTree.gss.
+        -- unfold nstates, DC.nstates in Hq. lia.
+        -- unfold DC.nstates. lia.
+        -- now rewrite (proj2 (Z.ltb_lt _ _)) by (unfold DC.nstates in Hq; lia).
+      * (* right conjunct *)
+        eapply eval_lt_test_gen with (j := s_idx) (bv := Int.one).
+        -- cbn - [Pos.add]. apply PTree.gss.
+        -- unfold DC.nsyms in Hs. lia.
+        -- unfold DC.nsyms. lia.
+        -- now rewrite (proj2 (Z.ltb_lt _ _)).
+      * (* sem_binary_operation Oand *)
+        cbn. unfold sem_and, sem_binarith, sem_cast, classify_cast,
+                    classify_binarith, tint. cbn.
+        destruct Archi.ptr64; cbn; reflexivity.
+    + apply bool_val_one_int.
+    + eapply exec_Sreturn_some.
+      eapply eval_Elvalue.
+      * (* eval_lvalue of the Ederef *)
+        econstructor.   (* eval_Ederef: needs eval_expr of the Ebinop *)
+        econstructor.   (* eval_Ebinop *)
+        -- (* Evar table decays to Vptr tb 0 *)
+           eapply eval_Elvalue.
+             eapply eval_Evar_global.
+               apply PTree.gempty.
+               exact Hsym.
+             eapply deref_loc_reference. reflexivity.
+        -- (* q * |Sigma| + s *)
+           unfold table_index.
+           assert (Hqb : 0 <= q_idx <= Int64.max_unsigned).
+             { pose proof nstates_bound. unfold DC.nstates in Hq. lia. }
+           assert (Hsb : 0 <= s_idx <= Int64.max_unsigned).
+             { pose proof nsyms_bound. unfold nsyms, DC.nsyms in Hs.
+              unfold Int64.max_unsigned. lia. }
+           assert (Hmb : 0 <= q_idx * DC.nsyms <= Int64.max_unsigned).
+             { pose proof nsyms_bound. pose proof ptrofs_le_int64.
+               unfold DC.nstates, DC.nsyms, Int64.max_unsigned in *. nia. }
+           econstructor.
+           ++ econstructor.
+              ** econstructor. cbn - [Pos.add].
+                 rewrite PTree.gso by (cbv [ids alloc_idents id_q id_s]; lia).
+                 apply PTree.gss.
+              ** econstructor.
+              ** cbn. unfold sem_mul, sem_binarith, sem_cast, classify_cast,
+                             classify_binarith, tlong. cbn.
+                 destruct Archi.ptr64; cbn;
+                   rewrite mul_repr_in_range by (assumption || apply nsyms_bound);
+                   reflexivity.
+           ++ econstructor. cbn - [Pos.add]. apply PTree.gss.
+           ++ cbn. unfold sem_add, classify_add, tlong. cbn.
+              unfold sem_binarith, sem_cast, classify_cast, classify_binarith. cbn.
+              destruct Archi.ptr64; cbn;
+                rewrite add_repr_in_range by assumption;
+                reflexivity.
+        -- (* sem_add: table + 8*(q*|Sigma|+s) *)
+           cbn. unfold sem_add, classify_add, table_type, tlong. cbn.
+           destruct Archi.ptr64 eqn:E; [|discriminate].
+           unfold sem_add_ptr_long. cbn.
+           do 2 f_equal.
+      * (* deref_loc: the actual load *)
+        eapply deref_loc_value with (chunk := Mint64).
+          reflexivity.
+        change Ptrofs.zero with (Ptrofs.repr 0).
+        rewrite ptr_add_normalize by
+          (pose proof ptrofs_le_int64; unfold DC.nstates, DC.nsyms in *; nia).
+        rewrite Z.add_0_l.
+        eapply table_in_mem.
+        -- exact Hsym.
+        -- apply table_entry_correct; eassumption.
+        -- unfold DC.nstates, DC.nsyms in *. nia.
   - cbn. split. discriminate.
-    unfold tlong, sem_cast, classify_cast.
-    now destruct Archi.ptr64; simpl.
+    unfold tlong, sem_cast, classify_cast. destruct Archi.ptr64; simpl;
+      now rewrite (table_entry_sidx q sym next_idx H1).
   - reflexivity.
 Qed.
 
@@ -484,33 +751,42 @@ Qed.
 
 (** delta returns the sink on out-of-range indices *)
 
-Lemma compile_delta_sink :
-  forall base q_idx s_idx m,
-    0 <= q_idx < Int64.modulus ->
-    q_idx >= Z.of_nat (length dfa.(states _)) ->
-    eval_funcall function_entry2 ge m
-      (compile_delta state dfa state_eq_dec (alloc_idents base))
-      [Vlong (Int64.repr q_idx); Vlong (Int64.repr s_idx)] E0 m
-      (Vlong (Int64.repr (sink_index state dfa))).
+Lemma compile_delta_sink : forall q_idx s_idx m,
+  0 <= q_idx < Int64.modulus ->
+  0 <= s_idx < Int64.modulus ->
+  q_idx >= DC.nstates state dfa ->
+  eval_funcall function_entry2 ge m
+    (compile_delta state dfa ids)
+    [Vlong (Int64.repr q_idx); Vlong (Int64.repr s_idx)] E0 m
+    (Vlong (Int64.repr (sink_index state dfa))).
 Proof.
-  intros. unfold compile_delta.
+  intros q_idx s_idx m Hq Hs Hoob.
   econstructor.
-  - econstructor; cbn - [Pos.succ Pos.add]; try solve [constructor].
+  - econstructor; cbn - [Pos.add]; try solve [constructor].
       apply alloc_idents_norepet.
       now repeat intro.
-  - cbn [fn_body]. apply fold_left_preserves_head.
-      econstructor. econstructor.
-    intros. destruct b as (qi & qq). econstructor.
-      eapply eval_eq_test_false; eauto.
-        cbn - [Pos.succ Pos.add]. rewrite PTree.gso by lia.
-          now rewrite PTree.gss.
-        pose proof (enumerate_In_bounds _ _ _ _ H1). lia.
-        intro. subst.
-          pose proof (enumerate_In_bounds _ _ _ _ H1). lia.
-      apply bool_val_zero.
-      assumption.
+  - cbn [fn_body]. eapply exec_Sifthenelse with (b := false).
+    + (* guard: (q < |Q|) & (s < |Sigma|) evaluates to Int.zero *)
+      econstructor.
+      * eapply eval_lt_test_gen with (j := q_idx) (bv := Int.zero).
+        -- cbn - [Pos.add].
+           rewrite PTree.gso by (cbv [ids alloc_idents id_q id_s]; lia).
+           apply PTree.gss.
+        -- assumption.
+        -- pose proof nstates_bound. unfold Int64.max_unsigned in *. lia.
+        -- now rewrite (proj2 (Z.ltb_ge _ _)) by lia.
+      * eapply eval_lt_test_gen with (j := s_idx).
+        -- cbn - [Pos.add]. apply PTree.gss.
+        -- assumption.
+        -- pose proof nsyms_bound. unfold Int64.max_unsigned in *. lia.
+        -- reflexivity.
+      * cbn. unfold sem_and, sem_binarith, sem_cast, classify_cast,
+                    classify_binarith, tint. cbn.
+        destruct Archi.ptr64; cbn; destruct (s_idx <? DC.nsyms); reflexivity.
+    + apply bool_val_zero_int.
+    + eapply exec_Sreturn_some. econstructor.
   - cbn. split. discriminate.
-    unfold sem_cast, tlong, classify_cast. now destruct Archi.ptr64.
+    unfold tlong, sem_cast, classify_cast. now destruct Archi.ptr64.
   - reflexivity.
 Qed.
 
@@ -546,16 +822,15 @@ Proof.
   now rewrite fold_left_app.
 Qed.
 
-Lemma delta_step_correct :
-  forall base w a q_idx a_idx m,
-    sidx (DFA.run dfa w) = Some q_idx ->
-    symidx a = Some a_idx ->
-    exists r_idx,
-      sidx (DFA.run dfa (w ++ [a])) = Some r_idx /\
-      eval_funcall function_entry2 ge m
-        (compile_delta state dfa state_eq_dec (alloc_idents base))
-        [Vlong (Int64.repr q_idx); Vlong (Int64.repr a_idx)] E0 m
-        (Vlong (Int64.repr r_idx)).
+Lemma delta_step_correct : forall w a q_idx a_idx,
+  sidx (DFA.run dfa w) = Some q_idx ->
+  symidx a = Some a_idx ->
+  exists r_idx,
+    sidx (DFA.run dfa (w ++ [a])) = Some r_idx /\
+    eval_funcall function_entry2 ge m0
+      (compile_delta state dfa ids)
+      [Vlong (Int64.repr q_idx); Vlong (Int64.repr a_idx)] E0 m0
+      (Vlong (Int64.repr r_idx)).
 Proof.
   intros. destruct (sidx_run (w ++ [a])).
   exists x. split.
@@ -574,6 +849,308 @@ Proof.
     apply (dfa.(states_complete _) []).
   destruct (index_of_complete _ _ 0 state_eq_dec Hin) as [i Hi].
   congruence.
+Qed.
+
+Lemma q0_index_bounds :
+  0 <= q0_index state dfa state_eq_dec < Int64.modulus.
+Proof.
+  pose proof q0_index_correct as H. unfold sidx in H.
+  apply index_of_bounds in H. lia.
+Qed.
+
+Definition sym_indices (w : list s.t) (l : list Z) : Prop :=
+  Forall2 (fun a i => symidx a = Some i) w l.
+
+Definition word_in_mem (m : mem) (b : block) (ofs : Z) (l : list Z) : Prop :=
+  forall n i, nth_error l n = Some i ->
+    Mem.loadv Mint64 m (Vptr b (Ptrofs.repr (ofs + 8 * Z.of_nat n)))
+      = Some (Vlong (Int64.repr i)).
+
+Lemma sym_indices_length : forall w l,
+  sym_indices w l -> length w = length l.
+Proof. intros. eapply Forall2_length; eassumption. Qed.
+
+Lemma sym_indices_bounds : forall w l i,
+  sym_indices w l -> In i l -> 0 <= i < Int64.modulus.
+Proof.
+  induction 1; intros. contradiction.
+  destruct H1; subst.
+    unfold symidx in H. apply index_of_bounds in H. lia.
+  eauto.
+Qed.
+
+Lemma sym_indices_nth : forall w l n a,
+  sym_indices w l ->
+  nth_error w n = Some a ->
+  exists i, nth_error l n = Some i /\ symidx a = Some i.
+Proof.
+  induction w; intros; destruct n; cbn in *; try discriminate;
+    inversion H; inversion H0; subst; eauto.
+Qed.
+
+(* Pointer arithmetic *)
+
+Lemma eval_index_lvalue : forall e le m b ofs i,
+  le ! (ids.(id_w)) = Some (Vptr b (Ptrofs.repr ofs)) ->
+  le ! (ids.(id_i)) = Some (Vlong (Int64.repr i)) ->
+  0 <= ofs -> 0 <= i -> ofs + 8 * i < Ptrofs.modulus ->
+  eval_lvalue ge e le m
+    (Ederef (Ebinop Oadd (Etempvar ids.(id_w) w_type) (Etempvar ids.(id_i) tlong) w_type) tlong)
+    b (Ptrofs.repr (ofs + 8 * i)) Full.
+Proof.
+  intros. econstructor. econstructor.
+    econstructor. eassumption.
+    econstructor. eassumption.
+  cbn.
+  destruct Archi.ptr64 eqn:E; [|discriminate].
+  f_equal. f_equal.
+  now apply ptr_add_normalize.
+Qed.
+
+(* Loop guard *)
+
+Lemma eval_lt_test : forall e le m i len bv,
+  le ! (ids.(id_i)) = Some (Vlong (Int64.repr i)) ->
+  le ! (ids.(id_len)) = Some (Vlong (Int64.repr len)) ->
+  0 <= i < Int64.modulus -> 0 <= len < Int64.modulus ->
+  bv = (if i <? len then Int.one else Int.zero) ->
+  eval_expr ge e le m
+    (Ebinop Olt (Etempvar ids.(id_i) tlong) (Etempvar ids.(id_len) tlong) tint)
+    (Vint bv).
+Proof.
+  intros. econstructor.
+    econstructor. eassumption.
+    econstructor. eassumption.
+  cbn. unfold sem_cmp, classify_cmp, tlong, sem_binarith, sem_cast,
+              classify_cast, classify_binarith. cbn.
+  destruct Archi.ptr64; cbn;
+    unfold Val.of_bool, Int64.ltu;
+    repeat rewrite Int64.unsigned_repr by (unfold Int64.max_unsigned; lia);
+    subst; destruct (i <? len) eqn:E;
+      [ rewrite zlt_true by lia | rewrite zlt_false by lia
+      | rewrite zlt_true by lia | rewrite zlt_false by lia ];
+      reflexivity.
+Qed.
+
+(* Loop body *)
+
+Definition run_body := run_body ids.
+Definition run_loop : statement := Sloop run_body Sskip.
+
+Lemma run_body_step : forall le m b ofs l i q_idx a_idx r_idx len,
+  le ! (ids.(id_w))   = Some (Vptr b (Ptrofs.repr ofs)) ->
+  le ! (ids.(id_len)) = Some (Vlong (Int64.repr len)) ->
+  le ! (ids.(id_i))   = Some (Vlong (Int64.repr i)) ->
+  le ! (ids.(id_q))   = Some (Vlong (Int64.repr q_idx)) ->
+  word_in_mem m b ofs l ->
+  nth_error l (Z.to_nat i) = Some a_idx ->
+  0 <= ofs -> 0 <= i < len -> len < Int64.modulus ->
+  ofs + 8 * i < Ptrofs.modulus ->
+  eval_funcall function_entry2 ge m
+    (compile_delta state dfa ids)
+    [Vlong (Int64.repr q_idx); Vlong (Int64.repr a_idx)] E0 m
+    (Vlong (Int64.repr r_idx)) ->
+  exec_stmt function_entry2 ge empty_env le m run_body E0
+    (PTree.set ids.(id_i) (Vlong (Int64.repr (i + 1)))
+      (PTree.set ids.(id_q) (Vlong (Int64.repr r_idx)) le))
+    m Out_normal.
+Proof.
+  intros. unfold run_body, DC.run_body.
+  change E0 with (E0 ** E0).
+  econstructor.
+  - econstructor.
+      eapply eval_lt_test with (bv := Int.one); eauto; try lia.
+        now rewrite (proj2 (Z.ltb_lt i len)) by lia.
+      apply bool_val_one_int.
+      constructor.
+  - change E0 with (E0 ** E0).
+    destruct find_delta as (loc & Sym & Funct). econstructor.
+    + (* q = delta(q, w[i]) *)
+      econstructor; eauto.
+      * reflexivity.
+      * (* the callee expression *)
+        eapply eval_Elvalue.
+          eapply eval_Evar_global.
+            apply PTree.gempty.
+            eassumption.
+          now eapply deref_loc_reference.
+      * (* the arguments *)
+        econstructor.
+          econstructor. eassumption.
+          cbn. unfold sem_cast, classify_cast, tlong. now destruct Archi.ptr64.
+        econstructor.
+          eapply eval_Elvalue.
+            eapply eval_index_lvalue; eauto; lia.
+          econstructor.
+            specialize (H3 (Z.to_nat i) a_idx H4).
+            rewrite Z2Nat.id in H3 by lia.
+            reflexivity.
+          specialize (H3 (Z.to_nat i) a_idx H4).
+            rewrite Z2Nat.id in H3 by lia. apply H3.
+          cbn. unfold sem_cast, classify_cast, tlong. now destruct Archi.ptr64.
+        econstructor.
+      * reflexivity.
+    + (* i = i + 1 *)
+      econstructor. econstructor.
+        econstructor.
+          rewrite PTree.gso by (cbv [ids alloc_idents id_i id_q]; lia).
+          eassumption.
+        econstructor.
+      cbn. unfold sem_binarith, sem_cast, classify_cast, classify_binarith, tlong. cbn.
+      destruct Archi.ptr64; cbn; do 2 f_equal;
+      rewrite Int64.add_unsigned;
+      rewrite !Int64.unsigned_repr by (unfold Int64.max_unsigned; lia);
+      reflexivity.
+Qed.
+
+Lemma run_loop_correct : forall suf pre l_pre l_suf b ofs le q_idx,
+  sym_indices pre l_pre ->
+  sym_indices suf l_suf ->
+  word_in_mem m0 b ofs (l_pre ++ l_suf) ->
+  sidx (DFA.run dfa pre) = Some q_idx ->
+  le ! (ids.(id_w))   = Some (Vptr b (Ptrofs.repr ofs)) ->
+  le ! (ids.(id_len)) = Some (Vlong (Int64.repr (Z.of_nat (length (pre ++ suf))))) ->
+  le ! (ids.(id_i))   = Some (Vlong (Int64.repr (Z.of_nat (length pre)))) ->
+  le ! (ids.(id_q))   = Some (Vlong (Int64.repr q_idx)) ->
+  0 <= ofs ->
+  Z.of_nat (length (pre ++ suf)) < Int64.modulus ->
+  ofs + 8 * Z.of_nat (length (pre ++ suf)) < Ptrofs.modulus ->
+  exists r_idx le',
+    sidx (DFA.run dfa (pre ++ suf)) = Some r_idx /\
+    le' ! (ids.(id_q)) = Some (Vlong (Int64.repr r_idx)) /\
+    exec_stmt function_entry2 ge empty_env le m0 run_loop E0 le' m0 Out_normal.
+Proof.
+  induction suf; intros.
+  - (* empty suffix: the guard fails and the loop breaks *)
+    exists q_idx, le. rewrite app_nil_r in *. repeat split; try assumption.
+    econstructor.
+      econstructor.
+        econstructor.
+          eapply eval_lt_test with (bv := Int.zero); eauto; try lia.
+            now rewrite (proj2 (Z.ltb_ge _ _)) by lia.
+          apply bool_val_zero_int.
+          constructor.
+        discriminate.
+    constructor.
+  - (* one iteration, then the loop at prefix [pre ++ [a]] *)
+    inversion H0; subst; clear H0.
+    pose proof (delta_step_correct pre a q_idx y H2 H12)
+      as (r_idx & Hr & Hcall).
+    assert (Hlp : length pre = length l_pre) by eauto using sym_indices_length.
+    assert (Hnth : nth_error (l_pre ++ y :: l') (Z.to_nat (Z.of_nat (length pre)))
+                   = Some y).
+      { rewrite Nat2Z.id, Hlp, nth_error_app2 by lia.
+        now rewrite Nat.sub_diag. }
+    edestruct (IHsuf (pre ++ [a]) (l_pre ++ [y]) l' b ofs
+      (PTree.set ids.(id_i) (Vlong (Int64.repr (Z.of_nat (length pre) + 1)))
+        (PTree.set ids.(id_q) (Vlong (Int64.repr r_idx)) le)) r_idx)
+      as (r' & le' & Hr' & Hq' & Hexec); eauto.
+    + apply Forall2_app; [assumption|now constructor].
+    + now rewrite <- app_assoc.
+    + rewrite PTree.gso, PTree.gso by (cbv [ids alloc_idents id_w id_i id_q]; lia).
+      assumption.
+    + rewrite PTree.gso, PTree.gso by (cbv [ids alloc_idents id_len id_i id_q]; lia).
+      rewrite <- app_assoc. assumption.
+    + rewrite PTree.gss. rewrite length_app. cbn.
+      now replace (Z.of_nat (length pre) + 1) with (Z.of_nat (length pre + 1)) by lia.
+    + rewrite PTree.gso, PTree.gss by (cbv [ids alloc_idents id_i id_q]; lia).
+      reflexivity.
+    + now rewrite <- app_assoc.
+    + now rewrite <- app_assoc.
+    + exists r', le'. rewrite <- app_assoc in Hr'. repeat split; eauto.
+      unfold run_loop.
+      change E0 with (E0 ** E0 ** E0).
+      eapply exec_Sloop_loop with (out1 := Out_normal).
+      * eapply run_body_step with (l := l_pre ++ y :: l')
+          (a_idx := y) (r_idx := r_idx); eauto;
+          rewrite length_app in *; cbn - [Pos.succ Pos.add Z.mul] in *; try lia.
+      * constructor.
+      * constructor.
+      * assumption.
+Qed.
+
+(* run *)
+
+Lemma alloc_idents_run_norepet :
+  list_norepet [ids.(id_w); ids.(id_len)] /\
+  list_norepet [ids.(id_i); ids.(id_q)] /\
+  list_disjoint [ids.(id_w); ids.(id_len)] [ids.(id_i); ids.(id_q)].
+Proof.
+  cbv [ids alloc_idents id_w id_len id_i id_q].
+  repeat split.
+  - repeat constructor; cbn - [Pos.add]; intro H;
+      repeat (destruct H as [H|H]; [lia|]); contradiction.
+  - repeat constructor; cbn - [Pos.add]; intro H;
+      repeat (destruct H as [H|H]; [lia|]); contradiction.
+  - repeat intro. cbn - [Pos.add] in *.
+    repeat (destruct H as [H|H]; subst; try contradiction);
+    repeat (destruct H0 as [H0|H0]; subst; try contradiction); lia.
+Qed.
+
+Lemma compile_run_correct : forall w l b ofs,
+  sym_indices w l ->
+  word_in_mem m0 b ofs l ->
+  0 <= ofs ->
+  Z.of_nat (length w) < Int64.modulus ->
+  ofs + 8 * Z.of_nat (length w) < Ptrofs.modulus ->
+  exists r_idx,
+    sidx (DFA.run dfa w) = Some r_idx /\
+    eval_funcall function_entry2 ge m0
+      (compile_run state dfa state_eq_dec ids)
+      [Vptr b (Ptrofs.repr ofs); Vlong (Int64.repr (Z.of_nat (length w)))] E0 m0
+      (Vlong (Int64.repr r_idx)).
+Proof.
+  intros. destruct alloc_idents_run_norepet, H5.
+  (* [le0]: the temp env after [function_entry2] binds the parameters. *)
+  set (le0 := PTree.set ids.(id_len) (Vlong (Int64.repr (Z.of_nat (length w))))
+               (PTree.set ids.(id_w) (Vptr b (Ptrofs.repr ofs))
+                 (create_undef_temps [(ids.(id_i), tlong); (ids.(id_q), tlong)]))).
+  (* [le1]: after the prologue sets [i := 0] and [q := q0]. *)
+  set (le1 := PTree.set ids.(id_q) (Vlong (Int64.repr (q0_index state dfa state_eq_dec)))
+               (PTree.set ids.(id_i) (Vlong (Int64.repr 0)) le0)).
+  assert (Hw1 : le1 ! (ids.(id_w)) = Some (Vptr b (Ptrofs.repr ofs))).
+    { subst le1 le0.
+      rewrite PTree.gso, PTree.gso by (cbv [ids alloc_idents id_w id_i id_q]; lia).
+      rewrite PTree.gso by (cbv [ids alloc_idents id_w id_len]; lia).
+      apply PTree.gss. }
+  assert (Hlen1 : le1 ! (ids.(id_len))
+                  = Some (Vlong (Int64.repr (Z.of_nat (length w))))).
+    { subst le1 le0.
+      rewrite PTree.gso, PTree.gso by (cbv [ids alloc_idents id_len id_i id_q]; lia).
+      apply PTree.gss. }
+  assert (Hi1 : le1 ! (ids.(id_i)) = Some (Vlong (Int64.repr 0))).
+    { subst le1.
+      rewrite PTree.gso by (cbv [ids alloc_idents id_i id_q]; lia).
+      apply PTree.gss. }
+  assert (Hq1 : le1 ! (ids.(id_q))
+                = Some (Vlong (Int64.repr (q0_index state dfa state_eq_dec)))).
+    { subst le1. apply PTree.gss. }
+  edestruct (run_loop_correct w [] [] l b ofs le1
+    (q0_index state dfa state_eq_dec)) as (r_idx & le' & Hr & Hq & Hexec); eauto.
+  - constructor.
+  - unfold run. simpl. apply q0_index_correct.
+  - cbn - [Pos.add] in *.
+    exists r_idx. split.
+      assumption.
+    unfold compile_run. econstructor.
+    + (* function_entry2 *)
+      econstructor; cbn - [Pos.add]; assumption || constructor.
+    + unfold DC.run_body. cbn [fn_body].
+      change E0 with (E0 ** E0).
+      eapply exec_Sseq_1.
+      * (* prologue ; loop *)
+        change E0 with (E0 ** E0).
+        eapply exec_Sseq_1.
+        -- (* Sset i 0 ; Sset q q0 *)
+           change E0 with (E0 ** E0).
+           eapply exec_Sseq_1.
+            econstructor. econstructor.
+            econstructor. unfold compiled_q0. econstructor.
+        -- eassumption.
+      * eapply exec_Sreturn_some. econstructor. eassumption.
+    + cbn. split. discriminate.
+      unfold tlong, sem_cast, classify_cast. now destruct Archi.ptr64.
+    + reflexivity.
 Qed.
 
 End correctness.
